Kami/Ex/ProcFDInl.v
@@ -8,24 +8,11 @@ Set Implicit Arguments.
 Section Inlined.
   Variables addrSize iaddrSize instBytes dataBytes rfIdx: nat.
 
-  (* External abstract ISA: decoding and execution *)
-  Variables (getOptype: OptypeT instBytes)
-            (getLdDst: LdDstT instBytes rfIdx)
-            (getLdAddr: LdAddrT addrSize instBytes)
-            (getLdSrc: LdSrcT instBytes rfIdx)
-            (calcLdAddr: LdAddrCalcT addrSize dataBytes)
-            (getStAddr: StAddrT addrSize instBytes)
-            (getStSrc: StSrcT instBytes rfIdx)
-            (calcStAddr: StAddrCalcT addrSize dataBytes)
-            (getStVSrc: StVSrcT instBytes rfIdx)
-            (getSrc1: Src1T instBytes rfIdx)
-            (getSrc2: Src2T instBytes rfIdx)
-            (getDst: DstT instBytes rfIdx)
-            (exec: ExecT iaddrSize instBytes dataBytes)
-            (getNextPc: NextPcT iaddrSize instBytes dataBytes rfIdx)
-            (alignInst: AlignInstT instBytes dataBytes)
-            (predictNextPc: forall ty, fullType ty (SyntaxKind (Pc iaddrSize)) -> (* pc *)
-                                       Expr ty (SyntaxKind (Pc iaddrSize))).
+  Variables (fetch: AbsFetch instBytes dataBytes)
+            (dec: AbsDec addrSize instBytes dataBytes rfIdx).
+
+  Variable predictNextPc: forall ty, fullType ty (SyntaxKind (Pc iaddrSize)) -> (* pc *)
+                                     Expr ty (SyntaxKind (Pc iaddrSize)).
 
   Variable (d2eElt: Kind).
   Variable (d2ePack:
@@ -61,10 +48,7 @@ Section Inlined.
 
   Variables (pcInit : ConstT (Pc iaddrSize)).
 
-  Definition fetchDecode := fetchDecode "rqFromProc"%string "rsToProc"%string
-                                        getOptype getLdDst getLdAddr getLdSrc calcLdAddr
-                                        getStAddr getStSrc calcStAddr getStVSrc
-                                        getSrc1 getSrc2 getDst alignInst predictNextPc
+  Definition fetchDecode := fetchDecode fetch dec predictNextPc
                                         d2ePack f2dPack f2dRawInst f2dCurPc f2dNextPc f2dEpoch
                                         pcInit.
   Hint Unfold fetchDecode: ModuleDefs. (* for kinline_compute *)
@@ -72,11 +56,8 @@ Section Inlined.
   Definition fetchDecodeInl: sigT (fun m: Modules => fetchDecode <<== m).
   Proof.
     pose proof (inlineF_refines
-                  (fetchDecode_ModEquiv "rqFromProc"%string "rsToProc"%string
-                                        getOptype getLdDst getLdAddr getLdSrc calcLdAddr
-                                        getStAddr getStSrc calcStAddr getStVSrc
-                                        getSrc1 getSrc2 getDst alignInst predictNextPc d2ePack
-                                        f2dPack f2dRawInst f2dCurPc f2dNextPc f2dEpoch
+                  (fetchDecode_ModEquiv fetch dec predictNextPc
+                                        d2ePack f2dPack f2dRawInst f2dCurPc f2dNextPc f2dEpoch
                                         pcInit type typeUT)
                   (Reflection.noDupStr_NoDup (Struct.namesOf (getDefsBodies fetchDecode)) eq_refl))
       as Him.
