Kami/Ex/ProcThreeStInl.v
@@ -7,24 +7,12 @@ Set Implicit Arguments.
 Section Inlined.
   Variables addrSize iaddrSize instBytes dataBytes rfIdx: nat.
 
-  (* External abstract ISA: decoding and execution *)
-  Variables (getOptype: OptypeT instBytes)
-            (getLdDst: LdDstT instBytes rfIdx)
-            (getLdAddr: LdAddrT addrSize instBytes)
-            (getLdSrc: LdSrcT instBytes rfIdx)
-            (calcLdAddr: LdAddrCalcT addrSize dataBytes)
-            (getStAddr: StAddrT addrSize instBytes)
-            (getStSrc: StSrcT instBytes rfIdx)
-            (calcStAddr: StAddrCalcT addrSize dataBytes)
-            (getStVSrc: StVSrcT instBytes rfIdx)
-            (getSrc1: Src1T instBytes rfIdx)
-            (getSrc2: Src2T instBytes rfIdx)
-            (getDst: DstT instBytes rfIdx)
-            (exec: ExecT iaddrSize instBytes dataBytes)
-            (getNextPc: NextPcT iaddrSize instBytes dataBytes rfIdx)
-            (alignInst: AlignInstT instBytes dataBytes)
-            (predictNextPc: forall ty, fullType ty (SyntaxKind (Pc iaddrSize)) -> (* pc *)
-                                       Expr ty (SyntaxKind (Pc iaddrSize))).
+  Variables (fetch: AbsFetch instBytes dataBytes)
+            (dec: AbsDec addrSize instBytes dataBytes rfIdx)
+            (exec: AbsExec iaddrSize instBytes dataBytes rfIdx).
+
+  Variable predictNextPc: forall ty, fullType ty (SyntaxKind (Pc iaddrSize)) -> (* pc *)
+                                     Expr ty (SyntaxKind (Pc iaddrSize)).
 
   Variable (d2eElt: Kind).
   Variable (d2ePack:
@@ -71,9 +59,7 @@ Section Inlined.
 
   Variable (init: ProcInit iaddrSize dataBytes rfIdx).
 
-  Definition p3st := p3st getOptype getLdDst getLdAddr getLdSrc calcLdAddr
-                          getStAddr getStSrc calcStAddr getStVSrc
-                          getSrc1 getSrc2 getDst exec getNextPc alignInst predictNextPc
+  Definition p3st := p3st fetch dec exec predictNextPc
                           d2ePack d2eOpType d2eDst d2eAddr d2eVal1 d2eVal2
                           d2eRawInst d2eCurPc d2eNextPc d2eEpoch
                           e2wPack e2wDecInst e2wVal init.
@@ -102,5 +88,6 @@ Section Inlined.
     exact (existT _ _ Him).
     END_SKIP_PROOF_ON *) apply cheat.
   Defined.
+
 End Inlined.
 
