Kami/Ex/ProcFDInv.v
@@ -12,24 +12,11 @@ Set Implicit Arguments.
 Section Invariants.
   Variables addrSize iaddrSize instBytes dataBytes rfIdx: nat.
 
-  (* External abstract ISA: decoding and execution *)
-  Variables (getOptype: OptypeT instBytes)
-            (getLdDst: LdDstT instBytes rfIdx)
-            (getLdAddr: LdAddrT addrSize instBytes)
-            (getLdSrc: LdSrcT instBytes rfIdx)
-            (calcLdAddr: LdAddrCalcT addrSize dataBytes)
-            (getStAddr: StAddrT addrSize instBytes)
-            (getStSrc: StSrcT instBytes rfIdx)
-            (calcStAddr: StAddrCalcT addrSize dataBytes)
-            (getStVSrc: StVSrcT instBytes rfIdx)
-            (getSrc1: Src1T instBytes rfIdx)
-            (getSrc2: Src2T instBytes rfIdx)
-            (getDst: DstT instBytes rfIdx)
-            (exec: ExecT iaddrSize instBytes dataBytes)
-            (getNextPc: NextPcT iaddrSize instBytes dataBytes rfIdx)
-            (alignInst: AlignInstT instBytes dataBytes)
-            (predictNextPc: forall ty, fullType ty (SyntaxKind (Pc iaddrSize)) -> (* pc *)
-                                       Expr ty (SyntaxKind (Pc iaddrSize))).
+  Variables (fetch: AbsFetch instBytes dataBytes)
+            (dec: AbsDec addrSize instBytes dataBytes rfIdx).
+
+  Variable predictNextPc: forall ty, fullType ty (SyntaxKind (Pc iaddrSize)) -> (* pc *)
+                                     Expr ty (SyntaxKind (Pc iaddrSize)).
 
   Variable (d2eElt: Kind).
   Variable (d2ePack:
@@ -79,9 +66,7 @@ Section Invariants.
   Variables (pcInit : ConstT (Pc iaddrSize)).
   
   Definition fetchDecodeInl := projT1 (fetchDecodeInl
-                                         getOptype getLdDst getLdAddr getLdSrc calcLdAddr
-                                         getStAddr getStSrc calcStAddr getStVSrc
-                                         getSrc1 getSrc2 getDst alignInst predictNextPc
+                                         fetch dec predictNextPc
                                          d2ePack f2dPack f2dRawInst f2dCurPc f2dNextPc f2dEpoch
                                          pcInit).
 
